Add imperative factorial

Stmt.v
@@ -2,20 +2,20 @@ Require Import List.
 Import ListNotations.
 Require Import Omega.
 
-Require Export BigZ.
+Require Export BinInt.
 Require Export Id.
 Require Export State.
 Require Export Expr.
 
 (* The type of statements *)
 Inductive stmt : Type :=
-  | SKIP  : stmt
-  | Assn  : id -> expr -> stmt
-  | READ  : id -> stmt
-  | WRITE : expr -> stmt
-  | Seq   : stmt -> stmt -> stmt
-  | If    : expr -> stmt -> stmt -> stmt
-  | While : expr -> stmt -> stmt.
+| SKIP  : stmt
+| Assn  : id -> expr -> stmt
+| READ  : id -> stmt
+| WRITE : expr -> stmt
+| Seq   : stmt -> stmt -> stmt
+| If    : expr -> stmt -> stmt -> stmt
+| While : expr -> stmt -> stmt.
 
 (* Supplementary notation *)
 Notation "x  '::=' e"                         := (Assn  x e    ) (at level 37, no associativity).
@@ -32,55 +32,195 @@ Reserved Notation "c1 '==' s '==>' c2" (at level 0).
 Notation "st [ x '<-' y ]" := (update Z st x y) (at level 0).
 
 Inductive bs_int : stmt -> conf -> conf -> Prop := 
-  | bs_Skip        : forall (c : conf), c == SKIP ==> c 
-  | bs_Assign      : forall (s : state Z) (i o : list Z) (x : id) (e : expr) (z : Z), 
-                       [| e |] s => z -> (s, i, o) == x ::= e ==> (s [x <- z], i, o)
-  | bs_Read        : forall (s : state Z) (i o : list Z) (x : id) (z : Z),
-                       (s, z::i, o) == READ x ==> (s [x <- z], i, o)
-  | bs_Write       : forall (s : state Z) (i o : list Z) (e : expr) (z : Z), 
-                       [| e |] s => z -> (s, i, o) == WRITE e ==> (s, i, z::o)
-  | bs_Seq         : forall (c c' c'' : conf) (s1 s2 : stmt),
-                       c == s1 ==> c' -> c' == s2 ==> c'' -> c ==  s1 ;; s2 ==> c''
-  | bs_If_True     : forall (s : state Z) (i o : list Z) (c' : conf) (e : expr) (s1 s2 : stmt),
-                       [| e |] s => Z.one -> (s, i, o) == s1 ==> c' -> (s, i, o) == COND e THEN s1 ELSE s2 END ==> c'
-  | bs_If_False    : forall (s : state Z) (i o : list Z) (c' : conf) (e : expr) (s1 s2 : stmt),
-                       [| e |] s => Z.zero -> (s, i, o) == s2 ==> c' -> (s, i, o) == COND e THEN s1 ELSE s2 END ==> c'
-  | bs_While_True  : forall (st : state Z) (i o : list Z) (c' c'' : conf) (e : expr) (s : stmt),
-                       [| e |] st => Z.one -> (st, i, o) == s ==> c' -> c' == WHILE e DO s END ==> c'' ->
-                          (st, i, o) == WHILE e DO s END ==> c''
-  | bs_While_False : forall (st : state Z) (i o : list Z) (e : expr) (s : stmt),
-                       [| e |] st => Z.zero -> (st, i, o) == WHILE e DO s END ==> (st, i, o)
+| bs_Skip        : forall (c : conf), c == SKIP ==> c 
+| bs_Assign      : forall (s : state Z) (i o : list Z) (x : id) (e : expr) (z : Z), 
+    [| e |] s => z -> (s, i, o) == x ::= e ==> (s [x <- z], i, o)
+| bs_Read        : forall (s : state Z) (i o : list Z) (x : id) (z : Z),
+    (s, z::i, o) == READ x ==> (s [x <- z], i, o)
+| bs_Write       : forall (s : state Z) (i o : list Z) (e : expr) (z : Z), 
+    [| e |] s => z -> (s, i, o) == WRITE e ==> (s, i, z::o)
+| bs_Seq         : forall (c c' c'' : conf) (s1 s2 : stmt),
+    c == s1 ==> c' -> c' == s2 ==> c'' -> c ==  s1 ;; s2 ==> c''
+| bs_If_True     : forall (s : state Z) (i o : list Z) (c' : conf) (e : expr) (s1 s2 : stmt),
+    [| e |] s => Z.one -> (s, i, o) == s1 ==> c' -> (s, i, o) == COND e THEN s1 ELSE s2 END ==> c'
+| bs_If_False    : forall (s : state Z) (i o : list Z) (c' : conf) (e : expr) (s1 s2 : stmt),
+    [| e |] s => Z.zero -> (s, i, o) == s2 ==> c' -> (s, i, o) == COND e THEN s1 ELSE s2 END ==> c'
+| bs_While_True  : forall (st : state Z) (i o : list Z) (c' c'' : conf) (e : expr) (s : stmt),
+    [| e |] st => Z.one -> (st, i, o) == s ==> c' -> c' == WHILE e DO s END ==> c'' ->
+                  (st, i, o) == WHILE e DO s END ==> c''
+| bs_While_False : forall (st : state Z) (i o : list Z) (e : expr) (s : stmt),
+    [| e |] st => Z.zero -> (st, i, o) == WHILE e DO s END ==> (st, i, o)
 where "c1 == s ==> c2" := (bs_int s c1 c2).
 
+Hint Constructors bs_int.
+
+
 (* Big-step semantics is deterministic *)
-Lemma bs_int_deterministic : forall (c c1 c2 : conf) (s : stmt), c == s ==> c1 -> c == s ==> c2 -> c1 = c2.
-Proof. admit. Admitted.
+Lemma bs_int_deterministic:
+  forall (c c1 c2 : conf) (s : stmt), c == s ==> c1 -> c == s ==> c2 -> c1 = c2.
+Proof.
+  intros.
+  generalize dependent c2.
+  induction H; intros c1 HYP. 
+  all: inversion_clear HYP.
+  all: try reflexivity.
+  all: try (match goal with
+            | H1: [| _ |] _ => (Z.zero), H2: [| _ |] _ => (Z.one)  |- _=>
+              exfalso; apply (bs_eval_deterministic _ _ _ _ H1) in H2; inversion H2  
+            end).
+  - apply (bs_eval_deterministic _ _ _ _ H) in H0; subst; reflexivity.
+  - apply (bs_eval_deterministic _ _ _ _ H) in H0; subst; reflexivity.
+  - apply IHbs_int1 in H1; subst.
+    apply IHbs_int2 in H2; subst. reflexivity.
+  - apply IHbs_int; assumption.
+  - apply IHbs_int; assumption.
+  - apply IHbs_int1 in H3; subst.
+    apply IHbs_int2 in H4; subst. reflexivity.
+Qed.
 
 Reserved Notation "s1 '~~~' s2" (at level 0).
 
 Inductive bs_equivalent: stmt -> stmt -> Prop :=
   bs_eq_intro: forall (s1 s2 : stmt), 
-                 (forall (c c' : conf), c == s1 ==> c' <-> c == s2 ==> c') -> s1 ~~~ s2
+    (forall (c c' : conf), c == s1 ==> c' <-> c == s2 ==> c') -> s1 ~~~ s2
 where "s1 '~~~' s2" := (bs_equivalent s1 s2).
 
 Module SmokeTest.
 
-  Lemma seq_assoc : forall (s1 s2 s3 : stmt) (c c' : conf),
-                      ((s1 ;; s2) ;; s3) ~~~ (s1 ;; (s2 ;; s3)).
-  Proof. admit. Admitted.
+  Lemma seq_assoc : forall (s1 s2 s3 : stmt),
+    ((s1 ;; s2) ;; s3) ~~~ (s1 ;; (s2 ;; s3)).
+  Proof.
+    intros; constructor; intros.
+    split; intros HYP.
+    { inversion_clear HYP; inversion_clear H.
+      eapply bs_Seq; eauto. 
+    } 
+    { inversion_clear HYP; inversion_clear H0.
+      eapply bs_Seq; eauto.
+    } 
+  Qed.      
 
-  Lemma while_unfolds : forall (e : expr) (s : stmt) (c c' : conf),
-                          (WHILE e DO s END) ~~~ (COND e THEN s ;; WHILE e DO s END ELSE SKIP END).
-  Proof. admit. Admitted.    
+  Lemma while_unfolds : forall (e : expr) (s : stmt),
+      (WHILE e DO s END) ~~~ (COND e THEN s ;; WHILE e DO s END ELSE SKIP END).
+  Proof.
+    intros; constructor; intros.
+    split; intros HYP.
+    { inversion_clear HYP.
+      apply bs_If_True; eauto. 
+      apply bs_If_False; eauto. 
+    }       
+    { inversion_clear HYP.
+      { inversion_clear H0.
+        eapply bs_While_True; eauto. }
+      { inversion H0. 
+        eapply bs_While_False; eauto. }
+    }
+  Qed.
 
   Lemma while_false : forall (e : expr) (s : stmt) (st : state Z) (i o : list Z) (c : conf),
-                        c == WHILE e DO s END ==> (st, i, o) -> [| e |] st => Z.zero.
-  Proof. admit. Admitted.
+      c == WHILE e DO s END ==> (st, i, o) -> [| e |] st => Z.zero.
+  Proof.
+  Admitted.
 
   Definition True := Nat 1.
 
-  Lemma loop_eq_undefined : (WHILE True DO SKIP END) ~~~ (COND (Nat 3) THEN SKIP ELSE SKIP END).
-  Proof. admit. Admitted.
+  Lemma loop_eq_undefined:
+    (WHILE True DO SKIP END) ~~~ (COND (Nat 3) THEN SKIP ELSE SKIP END).
+  Proof.
+    constructor; intros; split; intros.
+    inversion_clear H.
+
+    
+    induction H2.
+    
+    admit.
+  Admitted.
+
+  Fixpoint fact n :=
+    match n with
+    | 0 => 1
+    | S n => (S n) * fact n
+    end.
+
+  Let fact_imperative :=
+    (Id 0 ::= Nat 1);;
+    (READ (Id 1));;
+    (WHILE Var (Id 1) [>] Nat 0 DO
+      (Id 0 ::= (Var (Id 0) [*] Var (Id 1)));;
+      (Id 1 ::= (Var (Id 1) [-] Nat 1))
+    END);;
+    WRITE (Var (Id 0)).
+
+
+  Lemma fact_correct:
+    forall n, exists state_f,
+        (nil, [Z.of_nat n], nil) == fact_imperative ==> (state_f, nil, [Z.of_nat (fact n)]).
+  Proof.
+    assert (Fact1: Id 0 <> Id 1) by (intros CONTR; inversion CONTR).
+    assert (Fact2: Id 1 <> Id 0) by (intros CONTR; inversion CONTR).
+    intros n.
+    assert (
+        Fact: forall m state_s, exists state_f,
+            (((state_s [Id 0 <- m%Z]) [Id 1 <- Z.of_nat n], [], [])) ==
+            WHILE Var (Id 1) [>] Nat 0 DO
+              (Id 0 ::= (Var (Id 0) [*] Var (Id 1)));;
+              (Id 1 ::= (Var (Id 1) [-] Nat 1))
+            END ==> (state_f [Id 0 <- (m * Z.of_nat (fact n))%Z][Id 1 <- 0%Z],[],[])).
+    { induction n.
+      { intros; rewrite Z.mul_1_r.
+        exists state_s.
+        eapply bs_While_False, bs_Gt_F. 
+        - apply bs_Var, st_binds_hd.
+        - apply bs_Nat.
+        - apply Z.le_refl. 
+      }
+      intros.
+      specialize (IHn (m * Z.of_nat (S n))%Z).
+      specialize (IHn (((state_s) [Id 0 <- m]) [Id 1 <- Z.of_nat (S n)])).
+      destruct IHn as [state_f IHn].
+      exists state_f.
+      eapply bs_While_True.
+      { eapply bs_Gt_T.
+        - eapply bs_Var, st_binds_hd.
+        - apply bs_Nat.
+        - apply Zgt_pos_0. 
+      } 
+      { eapply bs_Seq.
+        { apply bs_Assign, bs_Mul.
+          - apply bs_Var, st_binds_tl; auto. 
+            apply st_binds_hd.
+          - apply bs_Var, st_binds_hd.
+        }
+        { apply bs_Assign, bs_Sub.
+          - apply bs_Var, st_binds_tl; auto.
+            apply st_binds_hd.
+          - apply bs_Nat.
+        }
+      }
+      { assert(EQ: (Z.of_nat (S n) - Z.of_nat 1)%Z = (Z.of_nat n)%Z).
+        { rewrite <- Nat2Z.inj_sub; simpl.
+          rewrite <- minus_n_O; auto.
+          apply Peano.le_n_S, Nat.le_0_l.
+        } rewrite EQ; clear EQ.
+        assert (EQ: (m * Z.of_nat (S n) * Z.of_nat (fact n))%Z =
+                    (m * Z.of_nat (fact (S n)))%Z).
+        { assert(F: fact (S n) = (S n) * fact n) by auto.
+          rewrite F; rewrite Nat2Z.inj_mul; rewrite Z.mul_assoc; auto.
+        } rewrite <- EQ; clear EQ.
+        apply IHn.
+      }
+    }
+    specialize (Fact 1%Z ([])); rewrite Z.mul_1_l in Fact.
+    destruct Fact as [state_f Fact].
+    exists (state_f[Id 0 <- Z.of_nat (fact n)][Id 1 <- 0%Z]).
+    eapply bs_Seq. apply bs_Assign; constructor.
+    eapply bs_Seq. eapply bs_Read; constructor.
+    eapply bs_Seq. apply Fact.
+    eapply bs_Write.
+    apply bs_Var.
+    apply st_binds_tl; auto.
+    apply st_binds_hd.
+  Qed.    
   
 End SmokeTest.
 
@@ -111,7 +251,7 @@ Reserved Notation "e1 '~c~' e2" (at level 42, no associativity).
 
 Inductive contextual_equivalent: stmt -> stmt -> Prop :=
   ceq_intro : forall (s1 s2 : stmt),
-                (forall (C : Context), (C <~ s1) ~~~ (C <~ s2)) -> s1 ~c~ s2
+    (forall (C : Context), (C <~ s1) ~~~ (C <~ s2)) -> s1 ~c~ s2
 where "s1 '~c~' s2" := (contextual_equivalent s1 s2).
 
 (* Contextual equivalence is equivalent to the semantic one *)
@@ -122,7 +262,7 @@ Proof. admit. Admitted.
 Inductive cont : Type := 
 | KEmpty : cont
 | KStmt  : stmt -> cont.
- 
+
 Definition Kapp (l r : cont) : cont :=
   match (l, r) with
   | (KStmt ls, KStmt rs) => KStmt (ls ;; rs)
@@ -138,44 +278,44 @@ Reserved Notation "k '|-' c1 '--' s '-->' c2" (at level 0).
 Inductive cps_int : cont -> cont -> conf -> conf -> Prop :=
 | cps_Empty       : forall (c : conf), KEmpty |- c -- KEmpty --> c
 | cps_Skip        : forall (c c' : conf) (k : cont), 
-                      KEmpty |- c -- k --> c' -> 
-                      k |- c -- !SKIP --> c'
+    KEmpty |- c -- k --> c' -> 
+              k |- c -- !SKIP --> c'
 | cps_Assn        : forall (s : state Z) (i o : list Z) (c' : conf) (k : cont) (x : id) (e : expr) (n : Z),
-                      [| e |] s => n ->
-                      KEmpty |- (s [x <- n], i, o) -- k --> c' ->
-                      k |- (s, i, o) -- !(x ::= e) --> c'
+    [| e |] s => n ->
+                 KEmpty |- (s [x <- n], i, o) -- k --> c' ->
+                           k |- (s, i, o) -- !(x ::= e) --> c'
 | cps_Read        : forall (s : state Z) (i o : list Z) (c' : conf) (k : cont) (x : id) (z : Z),
-                      KEmpty |- (s [x <- z], i, o) -- k --> c' ->
-                      k |- (s, z::i, o) -- !(READ x) --> c'
+    KEmpty |- (s [x <- z], i, o) -- k --> c' ->
+              k |- (s, z::i, o) -- !(READ x) --> c'
 | cps_Write       : forall (s : state Z) (i o : list Z) (c' : conf) (k : cont) (e : expr) (z : Z),
-                      [| e |] s => z ->
-                      KEmpty |- (s, i, z::o) -- k --> c' ->
-                      k |- (s, i, o) -- !(WRITE e) --> c'
+    [| e |] s => z ->
+                 KEmpty |- (s, i, z::o) -- k --> c' ->
+                           k |- (s, i, o) -- !(WRITE e) --> c'
 | cps_Seq         : forall (c c' : conf) (k : cont) (s1 s2 : stmt), 
-                      !s2 @ k |- c -- !s1 --> c' ->
-                      k |- c -- !(s1 ;; s2) --> c'
+    !s2 @ k |- c -- !s1 --> c' ->
+               k |- c -- !(s1 ;; s2) --> c'
 | cps_If_True     : forall (s : state Z) (i o : list Z) (c' : conf) (k : cont) (e : expr) (s1 s2 : stmt),
-                      [| e |] s => Z.one ->
-                      k |- (s, i, o) -- !s1 --> c' ->
+    [| e |] s => Z.one ->
+                 k |- (s, i, o) -- !s1 --> c' ->
                       k |- (s, i, o) -- !(COND e THEN s1 ELSE s2 END) --> c'
 | cps_If_False    : forall (s : state Z) (i o : list Z) (c' : conf) (k : cont) (e : expr) (s1 s2 : stmt),
-                      [| e |] s => Z.zero ->
-                      k |- (s, i, o) -- !s2 --> c' ->
+    [| e |] s => Z.zero ->
+                 k |- (s, i, o) -- !s2 --> c' ->
                       k |- (s, i, o) -- !(COND e THEN s1 ELSE s2 END) --> c'
 | cps_While_True  : forall (st : state Z) (i o : list Z) (c' : conf) (k : cont) (e : expr) (s : stmt),
-                      [| e |] st => Z.one ->
-                      !(WHILE e DO s END) @ k |- (st, i, o) -- !s --> c' ->
-                      k |- (st, i, o) -- !(WHILE e DO s END) --> c'
+    [| e |] st => Z.one ->
+                  !(WHILE e DO s END) @ k |- (st, i, o) -- !s --> c' ->
+                                             k |- (st, i, o) -- !(WHILE e DO s END) --> c'
 | cps_While_False : forall (st : state Z) (i o : list Z) (c' : conf) (k : cont) (e : expr) (s : stmt),
-                      [| e |] st => Z.zero ->
-                      KEmpty |- (st, i, o) -- k --> c' ->
-                      k |- (st, i, o) -- !(WHILE e DO s END) --> c'
+    [| e |] st => Z.zero ->
+                  KEmpty |- (st, i, o) -- k --> c' ->
+                            k |- (st, i, o) -- !(WHILE e DO s END) --> c'
 where "k |- c1 -- s --> c2" := (cps_int k s c1 c2).
 
 Lemma bs_int_to_cps_int: forall (st : state Z) (i o : list Z) (c' : conf) (s : stmt),
-  (st, i, o) == s ==> c' -> KEmpty |- (st, i, o) -- !s --> c'.
+    (st, i, o) == s ==> c' -> KEmpty |- (st, i, o) -- !s --> c'.
 Proof. admit. Admitted.
 
 Lemma cps_int_to_bs_int: forall (st : state Z) (i o : list Z) (c' : conf) (s : stmt),
-  KEmpty |- (st, i, o) -- !s --> c' -> (st, i, o) == s ==> c'.
+    KEmpty |- (st, i, o) -- !s --> c' -> (st, i, o) == s ==> c'.
 Proof. admit. Admitted.
